Std/Classes/Hashable.lean
@@ -1,0 +1,10 @@
+/-
+Copyright (c) 2018 Microsoft Corporation. All rights reserved.
+Released under Apache 2.0 license as described in the file LICENSE.
+Authors: Leonardo de Moura, Mario Carneiro
+-/
+
+/-- A hash is lawful if elements which compare equal under `==` have equal hash. -/
+class LawfulHashable (α : Type _) [BEq α] [Hashable α] : Prop where
+  /-- Two elements which compare equal under the `BEq` instance have equal hash. -/
+  hash_eq {a b : α} : a == b → hash a = hash b
