Std/Data/AssocList/WF.lean
@@ -1,0 +1,58 @@
+/-
+Copyright (c) 2024 Lean FRO, LLC. All rights reserved.
+Released under Apache 2.0 license as described in the file LICENSE.
+Authors: Markus Himmel
+-/
+import Std.Classes.BEq
+import Std.Classes.Hashable
+import Std.Data.AssocList
+
+set_option autoImplicit false
+
+universe u v
+
+variable {α : Type u} {β : Type v}
+
+namespace Std.AssocList
+
+/-- The well-formedness predicate for associative lists says that the keys are pairwise distinct. -/
+structure WF [BEq α] (l : AssocList α β) : Prop where
+  /-- The keys of a well-formed associative list are pairwise distinct. -/
+  distinct [PartialEquivBEq α] : l.keys.Pairwise fun a b => (a == b) = false
+
+@[simp]
+theorem WF.nil [BEq α] : (.nil : AssocList α β).WF :=
+  ⟨by simp⟩
+
+theorem WF.cons [BEq α] {l : AssocList α β} {k : α} {v : β} (h : l.contains k = false) :
+    l.WF → (l.cons k v).WF := sorry
+
+theorem WF.replace [BEq α] {l : AssocList α β} {k : α} {v : β} :
+    l.WF → (l.replace k v).WF := sorry
+
+/-- Well-formedness invariant for a bucket in a hash map. -/
+structure WFAtPosition [BEq α] [Hashable α] (l : AssocList α β) (i size : Nat)
+    extends l.WF : Prop where
+  /-- Every element in a bucket should hash to its location. -/
+  hash_self [LawfulHashable α] : ∀ k, l.contains k → ((hash k).toUSize % size).toNat = i
+
+@[simp]
+theorem WFAtPosition.nil [BEq α] [Hashable α] {i size} :
+    (.nil : AssocList α β).WFAtPosition i size :=
+  { WF.nil with
+    hash_self := by simp }
+
+theorem WFAtPosition.cons [BEq α] [Hashable α] {l : AssocList α β} {k : α} {v : β}
+    (h₁ : l.contains k = false) {i size : Nat} (h₂ : ((hash k).toUSize % size).toNat = i)
+    (h : l.WFAtPosition i size) : (l.cons k v).WFAtPosition i size :=
+  { h.toWF.cons h₁ with
+    hash_self := by
+      intros _ k'
+      sorry -- Okay, I need all of my normal forms from my own development
+    }
+
+theorem WFAtPosition.replace [BEq α] [Hashable α] {l : AssocList α β} {k : α} {v : β} {i size : Nat}
+    (h₁ : ((hash k).toUSize % size).toNat = i) (h : l.WFAtPosition i size) :
+    (l.replace k v).WFAtPosition i size := sorry
+
+end Std.AssocList
